$$F(\omega)=\frac{iR_sC_s\omega - L_sC_s\omega^2 + 1}{ i\omega (C_s + C_p)\left(\frac{iR_sC_pC_s\omega}{C_s + C_p} + 1 - \frac{C_sC_pL_s\omega^2}{C_s+C_p} \right)}$$

$$\begin{align}
A &= R_sC_s \\
B &= L_sC_s \\
C &= C_s + C_p \\
D &= C_sC_pL_s \\
E &= R_sC_pC_s
\end{align}$$

$$F(\omega)=\frac{iA\omega-B\omega^2+1}{i\omega C \left(\frac{iE}{C}\omega+1-\frac{D}{C}\omega^2 \right)}$$



$$\begin{align} \frac{\partial F}{\partial \omega}(\omega)=&\frac{i(\omega(D\omega(-2iA\omega+B\omega^2-3)+E(-A\omega+2i))+BC\omega^2+C)}{\omega^2(C+\omega(-D\omega+iE))^2}
\end{align}$$